Solution to the locking problem.

theories/examples/example.v
@@ -23,7 +23,7 @@ Set Primitive Projections.
 
 Import PackageNotation.
 
-Module SignatureDefs.
+Module Type SignatureDefs.
 
     Variable (n: nat).
     Definition pos_n: nat := 2^n.
@@ -32,6 +32,11 @@ Module SignatureDefs.
     Definition PubKey : choice_type := chFin(mkpos pos_n).
 
     Parameter KeyGen : Seed -> (SecKey × PubKey).
+
+    #[local] Open Scope package_scope.
+    Parameter KeyGenM :
+      ∀ {L : {fset Location}} (sd : Seed),
+        code L [interface] (SecKey × PubKey).
 
 End SignatureDefs.
 
@@ -89,4 +94,82 @@ Module RemoteAttestation (π : SignatureDefs).
     eapply eq_rel_perf_ind_eq.
     simplify_eq_rel x.
     all: ssprove_code_simpl.
-    eapply rsame_head_alt.
+    Fail eapply rreflexivity_rule.
+    Fail ssprove_sync.
+    Fail eapply r_ret.
+    Check rpost_weaken_rule.
+    eapply rpost_weaken_rule.
+    1:{ eapply rreflexivity_rule. }
+    intros.
+    move: H1; case eq_a0: a₀ => [b₀ s₀]; move => eq_a1 //=.
+    move: eq_a1; case eq_a1: a₁ => [b₁ s₁]; move => eq_b_s.
+    by [injection eq_b_s => eq_s eq_b].
+  Qed.
+
+End RemoteAttestation.
+
+Module RemoteAttestationM (π : SignatureDefs).
+
+  Import π.
+
+  Notation " 'pubkey "    := PubKey      (in custom pack_type at level 2) : package_scope.
+  Notation " 'seckey "    := SecKey      (in custom pack_type at level 2) : package_scope.
+  Notation " 'seed "      := Seed        (in custom pack_type at level 2) : package_scope.
+
+  Definition pk_loc      : Location := (PubKey    ; 0%N).
+  Definition sk_loc      : Location := (SecKey    ; 1%N).
+  Definition key_gen   : nat := 42.
+  Definition KeyGen_locs := fset [:: pk_loc ; sk_loc ].
+  Definition KG_interface := [interface #val #[key_gen] : 'seed → 'pubkey ].
+
+  Definition KG_real :
+  package KeyGen_locs
+    [interface]
+    KG_interface
+  :=
+  [package
+    #def  #[key_gen] (sd : 'seed) : 'pubkey
+    {
+    '(sk,pk) ← KeyGenM sd ;;
+    ret pk
+    }
+  ].
+
+  Definition KG_ideal :
+  package KeyGen_locs
+    [interface]
+    KG_interface
+  :=
+  [package
+    #def  #[key_gen] (sd : 'seed) : 'pubkey
+    {
+    '(sk,pk) ← KeyGenM sd ;;
+    ret pk
+    }
+  ].
+
+  Definition mkpair {Lt Lf E}
+    (t: package Lt [interface] E)
+    (f: package Lf [interface] E):
+    loc_GamePair E :=
+    fun b => if b then {locpackage t} else {locpackage f}.
+
+  Definition KG_ind := @mkpair KeyGen_locs KeyGen_locs KG_interface KG_real KG_ideal.
+
+  Lemma KG_real_vs_KG_true :
+  KG_ind true ≈₀ KG_ind false.
+  Proof.
+    eapply eq_rel_perf_ind_eq.
+    simplify_eq_rel x.
+    all: ssprove_code_simpl.
+    Fail eapply rsame_head.
+    Fail eapply rsame_head_alt.
+    eapply rpost_weaken_rule.
+    1:{ eapply rreflexivity_rule. }
+    intros.
+    move: H1; case eq_a0: a₀ => [b₀ s₀]; move => eq_a1 //=.
+    move: eq_a1; case eq_a1: a₁ => [b₁ s₁]; move => eq_b_s.
+    by [injection eq_b_s => eq_s eq_b].
+  Qed.
+
+End RemoteAttestationM.
